src/mqtt-packet-parser/src/ffi.fst
@@ -18,7 +18,9 @@ let zero_terminated_buffer_u8 (h: HS.mem) (b: B.buffer U8.t) = true
   // U8.v (Seq.index s (B.length b - 1)) = 0
 
 assume val uint8_to_c_string: u8_buffer: B.buffer U8.t -> Stack C.String.t
-  (requires (fun h -> B.live h u8_buffer /\ zero_terminated_buffer_u8 h u8_buffer /\ B.length u8_buffer = 65536))
+  (requires (fun h -> B.live h u8_buffer /\ 
+                      // zero_terminated_buffer_u8 h u8_buffer /\
+                      B.length u8_buffer = 65536))
   (ensures (fun h0 ret h1 -> U32.v (C.String.strlen ret) <= 65535))
 
 // assume val payload_uint8_to_c_string:
